spec+proofs: return new flag state after invokeSetFlags
This requires that the flags being set are first masked, to avoid
spurious flags that are unable to be represented by the types used in
the abstract.

Signed-off-by: Corey Lewis <corey.lewis@proofcraft.systems>

spec/haskell/src/SEL4/Object/Structures.lhs
@@ -501,6 +501,9 @@ Various operations on the free index of an Untyped cap.
 
 > data TcbFlag = FpuDisabled
 
+> numFlags :: Int
+> numFlags = 1
+
 > tcbFlagToWord :: TcbFlag -> Word
 > tcbFlagToWord (FpuDisabled) = bit 0
 
