proof/refine/AARCH64/Schedule_R.thy
@@ -1308,6 +1308,7 @@ lemma threadSet_invs_no_cicd'_trivialT:
     "\<forall>tcb. tcbDomain tcb \<le> maxDomain \<longrightarrow> tcbDomain (F tcb) \<le> maxDomain"
     "\<forall>tcb. tcbPriority tcb \<le> maxPriority \<longrightarrow> tcbPriority (F tcb) \<le> maxPriority"
     "\<forall>tcb. tcbMCP tcb \<le> maxPriority \<longrightarrow> tcbMCP (F tcb) \<le> maxPriority"
+    "\<forall>tcb. tcbFlags tcb \<le> mask numFlags \<longrightarrow> tcbFlags (F tcb) \<le> mask numFlags"
     "\<forall>tcb. atcbVCPUPtr (tcbArch (F tcb)) = atcbVCPUPtr (tcbArch tcb)"
   shows "threadSet F t \<lbrace>invs_no_cicd'\<rbrace>"
   apply (simp add: invs_no_cicd'_def valid_state'_def)
